src/arch/x64/X64.Leakage_Ins_Xmm_i.fst
@@ -29,10 +29,10 @@ let quad32_xor_lemma x =
   FStar.UInt.logxor_self #32 x.mid_hi;
   FStar.UInt.logxor_self #32 x.hi
 
-val check_if_pxor_leakage_free: (ins:tainted_ins{let i, _, _ = ins.ops in Pxor? i}) -> (fuel:nat) -> (ts:taintState) -> (res:(bool*taintState){let b, ts' = res in b2t b ==>
-     isConstantTime (Ins ins) fuel ts /\ isLeakageFree (Ins ins) fuel ts ts'})
+val check_if_pxor_leakage_free: (ins:tainted_ins{let i, _, _ = ins.ops in Pxor? i}) -> (ts:taintState) -> (res:(bool*taintState){let b, ts' = res in b2t b ==>
+     isConstantTime (Ins ins) ts /\ isLeakageFree (Ins ins) ts ts'})
 
-let check_if_pxor_leakage_free ins fuel ts =
+let check_if_pxor_leakage_free ins ts =
   let Pxor dst src, _, _ = ins.ops in
   if src = dst then begin
     let ts' = set_xmm_taint ts dst Public in
@@ -45,155 +45,156 @@ let check_if_pxor_leakage_free ins fuel ts =
     true, TaintState ts'.regTaint Secret ts'.xmmTaint
   end
 
-val check_if_paddd_leakage_free: (ins:tainted_ins{let i, _, _ = ins.ops in Paddd? i}) -> (fuel:nat) -> (ts:taintState) -> (res:(bool*taintState){let b, ts' = res in b2t b ==>
-     isConstantTime (Ins ins) fuel ts /\ isLeakageFree (Ins ins) fuel ts ts'})
+val check_if_paddd_leakage_free: (ins:tainted_ins{let i, _, _ = ins.ops in Paddd? i}) -> (ts:taintState) -> (res:(bool*taintState){let b, ts' = res in b2t b ==>
+     isConstantTime (Ins ins) ts /\ isLeakageFree (Ins ins) ts ts'})
 
-let check_if_paddd_leakage_free ins fuel ts =
+let check_if_paddd_leakage_free ins ts =
   let Paddd dst src, _, _ = ins.ops in
   let taint = merge_taint (xmm_taint ts dst) (xmm_taint ts src) in
   let ts' = set_xmm_taint ts dst taint in
   true, TaintState ts'.regTaint Secret ts'.xmmTaint
 
-val check_if_pslld_leakage_free: (ins:tainted_ins{let i, _, _ = ins.ops in Pslld? i}) -> (fuel:nat) -> (ts:taintState) -> (res:(bool*taintState){let b, ts' = res in b2t b ==>
-     isConstantTime (Ins ins) fuel ts /\ isLeakageFree (Ins ins) fuel ts ts'})
+val check_if_pslld_leakage_free: (ins:tainted_ins{let i, _, _ = ins.ops in Pslld? i}) -> (ts:taintState) -> (res:(bool*taintState){let b, ts' = res in b2t b ==>
+     isConstantTime (Ins ins) ts /\ isLeakageFree (Ins ins) ts ts'})
 
-let check_if_pslld_leakage_free ins fuel ts =
+let check_if_pslld_leakage_free ins ts =
   let Pslld dst amt, _, _ = ins.ops in
   let taint = xmm_taint ts dst in
   let ts' = set_xmm_taint ts dst taint in
   true, TaintState ts'.regTaint Secret ts'.xmmTaint
 
-val check_if_psrld_leakage_free: (ins:tainted_ins{let i, _, _ = ins.ops in Psrld? i}) -> (fuel:nat) -> (ts:taintState) -> (res:(bool*taintState){let b, ts' = res in b2t b ==>
-     isConstantTime (Ins ins) fuel ts /\ isLeakageFree (Ins ins) fuel ts ts'})
+val check_if_psrld_leakage_free: (ins:tainted_ins{let i, _, _ = ins.ops in Psrld? i}) -> (ts:taintState) -> (res:(bool*taintState){let b, ts' = res in b2t b ==>
+     isConstantTime (Ins ins) ts /\ isLeakageFree (Ins ins) ts ts'})
 
-let check_if_psrld_leakage_free ins fuel ts =
+let check_if_psrld_leakage_free ins ts =
   let Psrld dst amt, _, _ = ins.ops in
   let taint = xmm_taint ts dst in
   let ts' = set_xmm_taint ts dst taint in
   true, TaintState ts'.regTaint Secret ts'.xmmTaint
 
-val check_if_pshufb_leakage_free: (ins:tainted_ins{let i, _, _ = ins.ops in Pshufb? i}) -> (fuel:nat) -> (ts:taintState) -> (res:(bool*taintState){let b, ts' = res in b2t b ==>
-     isConstantTime (Ins ins) fuel ts /\ isLeakageFree (Ins ins) fuel ts ts'})
+val check_if_pshufb_leakage_free: (ins:tainted_ins{let i, _, _ = ins.ops in Pshufb? i}) -> (ts:taintState) -> (res:(bool*taintState){let b, ts' = res in b2t b ==>
+     isConstantTime (Ins ins) ts /\ isLeakageFree (Ins ins) ts ts'})
 
-let check_if_pshufb_leakage_free ins fuel ts =
+let check_if_pshufb_leakage_free ins ts =
   let Pshufb dst src, _, _ = ins.ops in
   let taint = merge_taint (xmm_taint ts dst) (xmm_taint ts src) in
   let ts' = set_xmm_taint ts dst taint in
   true, TaintState ts'.regTaint Secret ts'.xmmTaint
 
-val check_if_pshufd_leakage_free: (ins:tainted_ins{let i, _, _ = ins.ops in Pshufd? i}) -> (fuel:nat) -> (ts:taintState) -> (res:(bool*taintState){let b, ts' = res in b2t b ==>
-     isConstantTime (Ins ins) fuel ts /\ isLeakageFree (Ins ins) fuel ts ts'})
+val check_if_pshufd_leakage_free: (ins:tainted_ins{let i, _, _ = ins.ops in Pshufd? i}) -> (ts:taintState) -> (res:(bool*taintState){let b, ts' = res in b2t b ==>
+     isConstantTime (Ins ins) ts /\ isLeakageFree (Ins ins) ts ts'})
 
-let check_if_pshufd_leakage_free ins fuel ts =
+let check_if_pshufd_leakage_free ins ts =
   let Pshufd dst src _, _, _ = ins.ops in
   let taint = merge_taint (xmm_taint ts dst) (xmm_taint ts src) in
   let ts' = set_xmm_taint ts dst taint in
   true, TaintState ts'.regTaint Secret ts'.xmmTaint
 
-val check_if_pinsrd_leakage_free: (ins:tainted_ins{let i, _, _ = ins.ops in Pinsrd? i}) -> (fuel:nat) -> (ts:taintState) -> (res:(bool*taintState){let b, ts' = res in b2t b ==>
-     isConstantTime (Ins ins) fuel ts /\ isLeakageFree (Ins ins) fuel ts ts'})
+val check_if_pinsrd_leakage_free: (ins:tainted_ins{let i, _, _ = ins.ops in Pinsrd? i}) -> (ts:taintState) -> (res:(bool*taintState){let b, ts' = res in b2t b ==>
+     isConstantTime (Ins ins) ts /\ isLeakageFree (Ins ins) ts ts'})
 
-let check_if_pinsrd_leakage_free ins fuel ts =
+let check_if_pinsrd_leakage_free ins ts =
   let Pinsrd dst src _, _, _ = ins.ops in
   let fixedTime = operand_does_not_use_secrets src ts in
+  assert (fixedTime ==> isConstantTime (Ins ins) ts);
   let taint = merge_taint (xmm_taint ts dst) (operand_taint src ts) in
   let taint = merge_taint taint ins.t in
   let ts' = set_xmm_taint ts dst taint in
   fixedTime, TaintState ts'.regTaint Secret ts'.xmmTaint
 
-val check_if_vpslldq_leakage_free: (ins:tainted_ins{let i, _, _ = ins.ops in VPSLLDQ? i}) -> (fuel:nat) -> (ts:taintState) -> (res:(bool*taintState){let b, ts' = res in b2t b ==>
-     isConstantTime (Ins ins) fuel ts /\ isLeakageFree (Ins ins) fuel ts ts'})
+val check_if_vpslldq_leakage_free: (ins:tainted_ins{let i, _, _ = ins.ops in VPSLLDQ? i}) -> (ts:taintState) -> (res:(bool*taintState){let b, ts' = res in b2t b ==>
+     isConstantTime (Ins ins) ts /\ isLeakageFree (Ins ins) ts ts'})
 
-let check_if_vpslldq_leakage_free ins fuel ts =
+let check_if_vpslldq_leakage_free ins ts =
   let VPSLLDQ dst src _, _, _ = ins.ops in
   let taint = merge_taint (xmm_taint ts dst) (xmm_taint ts src) in
   let ts' = set_xmm_taint ts dst taint in
   true, TaintState ts'.regTaint Secret ts'.xmmTaint
 
-val check_if_pclmuldqd_leakage_free: (ins:tainted_ins{let i, _, _ = ins.ops in Pclmulqdq? i}) -> (fuel:nat) -> (ts:taintState) -> (res:(bool*taintState){let b, ts' = res in b2t b ==>
-     isConstantTime (Ins ins) fuel ts /\ isLeakageFree (Ins ins) fuel ts ts'})
+val check_if_pclmuldqd_leakage_free: (ins:tainted_ins{let i, _, _ = ins.ops in Pclmulqdq? i}) -> (ts:taintState) -> (res:(bool*taintState){let b, ts' = res in b2t b ==>
+     isConstantTime (Ins ins) ts /\ isLeakageFree (Ins ins) ts ts'})
 
 #set-options "--z3rlimit 40"
 
-let check_if_pclmuldqd_leakage_free ins fuel ts =
+let check_if_pclmuldqd_leakage_free ins ts =
   let Pclmulqdq dst src _, _, _ = ins.ops in
   let taint = merge_taint (xmm_taint ts dst) (xmm_taint ts src) in
   let ts' = set_xmm_taint ts dst taint in
   true, TaintState ts'.regTaint Secret ts'.xmmTaint
 
-val check_if_aesni_enc_leakage_free: (ins:tainted_ins{let i, _, _ = ins.ops in AESNI_enc? i}) -> (fuel:nat) -> (ts:taintState) -> (res:(bool*taintState){let b, ts' = res in b2t b ==>
-     isConstantTime (Ins ins) fuel ts /\ isLeakageFree (Ins ins) fuel ts ts'})
+val check_if_aesni_enc_leakage_free: (ins:tainted_ins{let i, _, _ = ins.ops in AESNI_enc? i}) -> (ts:taintState) -> (res:(bool*taintState){let b, ts' = res in b2t b ==>
+     isConstantTime (Ins ins) ts /\ isLeakageFree (Ins ins) ts ts'})
 
-let check_if_aesni_enc_leakage_free ins fuel ts =
+let check_if_aesni_enc_leakage_free ins ts =
   let AESNI_enc dst src, _, _ = ins.ops in
   let taint = merge_taint (xmm_taint ts dst) (xmm_taint ts src) in
   let ts' = set_xmm_taint ts dst taint in
   true, TaintState ts'.regTaint Secret ts'.xmmTaint
 
-val check_if_aesni_enc_last_leakage_free: (ins:tainted_ins{let i, _, _ = ins.ops in AESNI_enc_last? i}) -> (fuel:nat) -> (ts:taintState) -> (res:(bool*taintState){let b, ts' = res in b2t b ==>
-     isConstantTime (Ins ins) fuel ts /\ isLeakageFree (Ins ins) fuel ts ts'})
+val check_if_aesni_enc_last_leakage_free: (ins:tainted_ins{let i, _, _ = ins.ops in AESNI_enc_last? i}) -> (ts:taintState) -> (res:(bool*taintState){let b, ts' = res in b2t b ==>
+     isConstantTime (Ins ins) ts /\ isLeakageFree (Ins ins) ts ts'})
 
-let check_if_aesni_enc_last_leakage_free ins fuel ts =
+let check_if_aesni_enc_last_leakage_free ins ts =
   let AESNI_enc_last dst src, _, _ = ins.ops in
   let taint = merge_taint (xmm_taint ts dst) (xmm_taint ts src) in
   let ts' = set_xmm_taint ts dst taint in
   true, TaintState ts'.regTaint Secret ts'.xmmTaint
 
-val check_if_aesni_dec_leakage_free: (ins:tainted_ins{let i, _, _ = ins.ops in AESNI_dec? i}) -> (fuel:nat) -> (ts:taintState) -> (res:(bool*taintState){let b, ts' = res in b2t b ==>
-     isConstantTime (Ins ins) fuel ts /\ isLeakageFree (Ins ins) fuel ts ts'})
+val check_if_aesni_dec_leakage_free: (ins:tainted_ins{let i, _, _ = ins.ops in AESNI_dec? i}) -> (ts:taintState) -> (res:(bool*taintState){let b, ts' = res in b2t b ==>
+     isConstantTime (Ins ins) ts /\ isLeakageFree (Ins ins) ts ts'})
 
-let check_if_aesni_dec_leakage_free ins fuel ts =
+let check_if_aesni_dec_leakage_free ins ts =
   let AESNI_dec dst src, _, _ = ins.ops in
   let taint = merge_taint (xmm_taint ts dst) (xmm_taint ts src) in
   let ts' = set_xmm_taint ts dst taint in
   true, TaintState ts'.regTaint Secret ts'.xmmTaint
 
-val check_if_aesni_dec_last_leakage_free: (ins:tainted_ins{let i, _, _ = ins.ops in AESNI_dec_last? i}) -> (fuel:nat) -> (ts:taintState) -> (res:(bool*taintState){let b, ts' = res in b2t b ==>
-     isConstantTime (Ins ins) fuel ts /\ isLeakageFree (Ins ins) fuel ts ts'})
+val check_if_aesni_dec_last_leakage_free: (ins:tainted_ins{let i, _, _ = ins.ops in AESNI_dec_last? i}) -> (ts:taintState) -> (res:(bool*taintState){let b, ts' = res in b2t b ==>
+     isConstantTime (Ins ins) ts /\ isLeakageFree (Ins ins) ts ts'})
 
-let check_if_aesni_dec_last_leakage_free ins fuel ts =
+let check_if_aesni_dec_last_leakage_free ins ts =
   let AESNI_dec_last dst src, _, _ = ins.ops in
   let taint = merge_taint (xmm_taint ts dst) (xmm_taint ts src) in
   let ts' = set_xmm_taint ts dst taint in
   true, TaintState ts'.regTaint Secret ts'.xmmTaint
 
-val check_if_aesni_imc_leakage_free: (ins:tainted_ins{let i, _, _ = ins.ops in AESNI_imc? i}) -> (fuel:nat) -> (ts:taintState) -> (res:(bool*taintState){let b, ts' = res in b2t b ==>
-     isConstantTime (Ins ins) fuel ts /\ isLeakageFree (Ins ins) fuel ts ts'})
+val check_if_aesni_imc_leakage_free: (ins:tainted_ins{let i, _, _ = ins.ops in AESNI_imc? i}) -> (ts:taintState) -> (res:(bool*taintState){let b, ts' = res in b2t b ==>
+     isConstantTime (Ins ins) ts /\ isLeakageFree (Ins ins) ts ts'})
 
-let check_if_aesni_imc_leakage_free ins fuel ts =
+let check_if_aesni_imc_leakage_free ins ts =
   let AESNI_imc dst src, _, _ = ins.ops in
   let taint = merge_taint (xmm_taint ts dst) (xmm_taint ts src) in
   let ts' = set_xmm_taint ts dst taint in
   true, TaintState ts'.regTaint Secret ts'.xmmTaint
 
-val check_if_aesni_keygen_leakage_free: (ins:tainted_ins{let i, _, _ = ins.ops in AESNI_keygen_assist? i}) -> (fuel:nat) -> (ts:taintState) -> (res:(bool*taintState){let b, ts' = res in b2t b ==>
-     isConstantTime (Ins ins) fuel ts /\ isLeakageFree (Ins ins) fuel ts ts'})
+val check_if_aesni_keygen_leakage_free: (ins:tainted_ins{let i, _, _ = ins.ops in AESNI_keygen_assist? i}) -> (ts:taintState) -> (res:(bool*taintState){let b, ts' = res in b2t b ==>
+     isConstantTime (Ins ins) ts /\ isLeakageFree (Ins ins) ts ts'})
 
-let check_if_aesni_keygen_leakage_free ins fuel ts =
+let check_if_aesni_keygen_leakage_free ins ts =
   let AESNI_keygen_assist dst src _, _, _ = ins.ops in
   let taint = merge_taint (xmm_taint ts dst) (xmm_taint ts src) in
   let ts' = set_xmm_taint ts dst taint in
   true, TaintState ts'.regTaint Secret ts'.xmmTaint
 
-val check_if_xmm_ins_consumes_fixed_time: (ins:tainted_ins{is_xmm_ins ins}) -> (fuel:nat) -> (ts:taintState) -> (res:(bool*taintState){ins_consumes_fixed_time ins fuel ts res})
+val check_if_xmm_ins_consumes_fixed_time: (ins:tainted_ins{is_xmm_ins ins}) -> (ts:taintState) -> (res:(bool*taintState){ins_consumes_fixed_time ins ts res})
 
-let check_if_xmm_ins_consumes_fixed_time ins fuel ts =
+let check_if_xmm_ins_consumes_fixed_time ins ts =
   let i, _, _ = ins.ops in
   match i with
-    | Paddd dst src -> check_if_paddd_leakage_free ins fuel ts
-    | Pxor dst src -> check_if_pxor_leakage_free ins fuel ts
-    | Pslld dst amt -> check_if_pslld_leakage_free ins fuel ts
-    | Psrld dst amt -> check_if_psrld_leakage_free ins fuel ts
-    | Pshufb dst src -> check_if_pshufb_leakage_free ins fuel ts
-    | Pshufd dst src permutation -> check_if_pshufd_leakage_free ins fuel ts
-    | Pinsrd dst srx index -> check_if_pinsrd_leakage_free ins fuel ts
-    | VPSLLDQ dst src count -> check_if_vpslldq_leakage_free ins fuel ts
+    | Paddd dst src -> check_if_paddd_leakage_free ins ts
+    | Pxor dst src -> check_if_pxor_leakage_free ins ts
+    | Pslld dst amt -> check_if_pslld_leakage_free ins ts
+    | Psrld dst amt -> check_if_psrld_leakage_free ins ts
+    | Pshufb dst src -> check_if_pshufb_leakage_free ins ts
+    | Pshufd dst src permutation -> check_if_pshufd_leakage_free ins ts
+    | Pinsrd dst srx index -> check_if_pinsrd_leakage_free ins ts
+    | VPSLLDQ dst src count -> check_if_vpslldq_leakage_free ins ts
     | MOVDQU dst src -> false, ts
-    | Pclmulqdq dst src imm -> check_if_pclmuldqd_leakage_free ins fuel ts
-    | AESNI_enc dst src -> check_if_aesni_enc_leakage_free ins fuel ts
-    | AESNI_enc_last dst src -> check_if_aesni_enc_last_leakage_free ins fuel ts
-    | AESNI_dec dst src -> check_if_aesni_dec_leakage_free ins fuel ts
-    | AESNI_dec_last dst src -> check_if_aesni_dec_last_leakage_free ins fuel ts
-    | AESNI_imc dst src -> check_if_aesni_imc_leakage_free ins fuel ts
-    | AESNI_keygen_assist dst src imm -> check_if_aesni_keygen_leakage_free ins fuel ts
+    | Pclmulqdq dst src imm -> check_if_pclmuldqd_leakage_free ins ts
+    | AESNI_enc dst src -> check_if_aesni_enc_leakage_free ins ts
+    | AESNI_enc_last dst src -> check_if_aesni_enc_last_leakage_free ins ts
+    | AESNI_dec dst src -> check_if_aesni_dec_leakage_free ins ts
+    | AESNI_dec_last dst src -> check_if_aesni_dec_last_leakage_free ins ts
+    | AESNI_imc dst src -> check_if_aesni_imc_leakage_free ins ts
+    | AESNI_keygen_assist dst src imm -> check_if_aesni_keygen_leakage_free ins ts
     
