src/arch/x64/X64.Leakage_Ins_i.fst
@@ -10,18 +10,19 @@ open FStar.Tactics
 #reset-options "--initial_ifuel 2 --max_ifuel 2 --initial_fuel 4 --max_fuel 4 --using_facts_from '* -FStar.Reflection -FStar.Tactics'"
 
 
-val check_if_ins_consumes_fixed_time: (ins:tainted_ins{not (is_xmm_ins ins)}) -> (fuel:nat) -> (ts:taintState) -> (res:(bool*taintState){ins_consumes_fixed_time ins fuel ts res})
-#reset-options "--initial_ifuel 2 --max_ifuel 2 --initial_fuel 4 --max_fuel 4 --using_facts_from '* -FStar.Reflection -FStar.Tactics' --z3rlimit 30"
+val check_if_ins_consumes_fixed_time: (ins:tainted_ins{not (is_xmm_ins ins)}) -> (ts:taintState) -> (res:(bool*taintState){ins_consumes_fixed_time ins ts res})
+#reset-options "--initial_ifuel 2 --max_ifuel 2 --initial_fuel 4 --max_fuel 4 --using_facts_from '* -FStar.Reflection -FStar.Tactics' --z3rlimit 40"
 
-let check_if_ins_consumes_fixed_time ins fuel ts =
+
+let check_if_ins_consumes_fixed_time ins ts =
   let i, dsts, srcs = ins.ops in
   let ftSrcs = operands_do_not_use_secrets srcs ts in
   let ftDsts = operands_do_not_use_secrets dsts ts in
   let fixedTime = ftSrcs && ftDsts in
 
   Classical.forall_intro_2 (fun x y -> lemma_operand_obs_list ts dsts x y);
-  Classical.forall_intro_2 (lemma_operand_obs_list ts srcs);
-  assert (fixedTime ==> (isConstantTime (Ins ins) fuel ts));
+  Classical.forall_intro_2 (fun x y -> lemma_operand_obs_list ts srcs x y);
+  assert (fixedTime ==> (isConstantTime (Ins ins) ts));
   let taint = sources_taint srcs ts ins.t in
   let taint = if AddCarry64? i then merge_taint taint ts.flagsTaint else taint in
   let ts' = set_taints dsts ts taint in
@@ -33,31 +34,36 @@ let check_if_ins_consumes_fixed_time ins fuel ts =
 	| OMem m -> (fixedTime && (not (Secret? taint && Public? (operand_taint (OMem m) ts)))), ts'
     end
     | Mul64 _ -> fixedTime, (TaintState ts'.regTaint Secret ts'.xmmTaint)
-    | Xor64 dst src -> 
+    | Xor64 dst src ->
         (* Special case for Xor : xor-ing an operand with itself erases secret data *)
         if dst = src then
 	  let ts' = set_taint dst ts' Public in
 	  fixedTime, TaintState ts'.regTaint Secret ts'.xmmTaint
-        else begin match dst with
-	  | OConst _ -> false, ts (* Should not happen *)
+        else
+	begin match dst with
+	  | OConst _ -> false, (TaintState ts'.regTaint Secret ts'.xmmTaint) (* Should not happen *)
 	  | OReg r -> fixedTime, (TaintState ts'.regTaint Secret ts'.xmmTaint)
 	  | OMem m -> (fixedTime && (not (Secret? taint && Public? (operand_taint (OMem m) ts)))), (TaintState ts'.regTaint Secret ts'.xmmTaint)
         end
-    | _ -> 
+    | _ ->
       match dsts with
-	| [OConst _] -> false, ts (* Should not happen *)
+	| [OConst _] -> false, (TaintState ts'.regTaint Secret ts'.xmmTaint) (* Should not happen *)
 	| [OReg r] -> fixedTime, (TaintState ts'.regTaint Secret ts'.xmmTaint)
 	| [OMem m] ->  (fixedTime && (not (Secret? taint && Public? (operand_taint (OMem m) ts)))), (TaintState ts'.regTaint Secret ts'.xmmTaint)
   in
   b, ts'
 
-val lemma_mov_same_public: (ts:taintState) -> (fuel:nat) -> (ins:tainted_ins{let i, _, _ = ins.ops in Mov64? i}) -> (s1:traceState) -> (s2:traceState) -> Lemma
-(let b, ts' = check_if_ins_consumes_fixed_time ins fuel ts in
+val lemma_public_flags_same: (ts:taintState) -> (ins:tainted_ins{not (is_xmm_ins ins)}) -> Lemma (forall s1 s2. publicFlagValuesAreSame ts s1 s2 ==> publicFlagValuesAreSame (snd (check_if_ins_consumes_fixed_time ins ts)) (taint_eval_ins ins s1) (taint_eval_ins ins s2))
+
+let lemma_public_flags_same ts ins = ()
+
+val lemma_mov_same_public: (ts:taintState) -> (ins:tainted_ins{let i, _, _ = ins.ops in Mov64? i}) -> (s1:traceState) -> (s2:traceState) -> (fuel:nat) -> Lemma
+(let b, ts' = check_if_ins_consumes_fixed_time ins ts in
   (b2t b ==> isExplicitLeakageFreeGivenStates (Ins ins) fuel ts ts' s1 s2))
 
 #reset-options "--initial_ifuel 2 --max_ifuel 2 --initial_fuel 4 --max_fuel 4 --using_facts_from '* -FStar.Reflection -FStar.Tactics' --z3rlimit 80"
-let lemma_mov_same_public ts fuel ins s1 s2 =
-  let b, ts' = check_if_ins_consumes_fixed_time ins fuel ts in
+let lemma_mov_same_public ts ins s1 s2 fuel =
+  let b, ts' = check_if_ins_consumes_fixed_time ins ts in
   let i, dsts, srcs = ins.ops in
   let r1 = taint_eval_ins ins s1 in
   let r2 = taint_eval_ins ins s2 in
@@ -79,13 +85,13 @@ let lemma_mov_same_public ts fuel ins s1 s2 =
 	  lemma_frame_store_mem64 ptr2 v2 s2.state.mem;
           assert (b2t b /\ r1.state.ok /\ r2.state.ok /\ publicValuesAreSame ts s1 s2 ==> publicValuesAreSame ts' r1 r2) 
 
-val lemma_add_same_public: (ts:taintState) -> (fuel:nat) -> (ins:tainted_ins{let i, _, _ = ins.ops in Add64? i}) -> (s1:traceState) -> (s2:traceState) -> Lemma
-(let b, ts' = check_if_ins_consumes_fixed_time ins fuel ts in
+val lemma_add_same_public: (ts:taintState) -> (ins:tainted_ins{let i, _, _ = ins.ops in Add64? i}) -> (s1:traceState) -> (s2:traceState) -> (fuel:nat) -> Lemma
+(let b, ts' = check_if_ins_consumes_fixed_time ins ts in
   (b2t b ==> isExplicitLeakageFreeGivenStates (Ins ins) fuel ts ts' s1 s2))
 
 #reset-options "--z3cliopt smt.CASE_SPLIT=3 --initial_ifuel 2 --max_ifuel 2 --initial_fuel 4 --max_fuel 4 --using_facts_from '* -FStar.Reflection -FStar.Tactics' --z3rlimit 100"
-let lemma_add_same_public ts fuel ins s1 s2 =
-  let b, ts' = check_if_ins_consumes_fixed_time ins fuel ts in
+let lemma_add_same_public ts ins s1 s2 fuel =
+  let b, ts' = check_if_ins_consumes_fixed_time ins ts in
   let i, dsts, srcs = ins.ops in
   let r1 = taint_eval_ins ins s1 in
   let r2 = taint_eval_ins ins s2 in
@@ -111,12 +117,12 @@ let lemma_add_same_public ts fuel ins s1 s2 =
 	  lemma_frame_store_mem64 ptr2 v2 s2.state.mem;
 	  assert (b2t b /\ r1.state.ok /\ r2.state.ok /\ publicValuesAreSame ts s1 s2 ==> publicValuesAreSame ts' r1 r2)
 
-val lemma_sub_same_public: (ts:taintState) -> (fuel:nat) -> (ins:tainted_ins{let i, _, _ = ins.ops in Sub64? i}) -> (s1:traceState) -> (s2:traceState) -> Lemma
-(let b, ts' = check_if_ins_consumes_fixed_time ins fuel ts in
+val lemma_sub_same_public: (ts:taintState) -> (ins:tainted_ins{let i, _, _ = ins.ops in Sub64? i}) -> (s1:traceState) -> (s2:traceState) -> (fuel:nat) -> Lemma
+(let b, ts' = check_if_ins_consumes_fixed_time ins ts in
   (b2t b ==> isExplicitLeakageFreeGivenStates (Ins ins) fuel ts ts' s1 s2))
 
-let lemma_sub_same_public ts fuel ins s1 s2 =
-  let b, ts' = check_if_ins_consumes_fixed_time ins fuel ts in
+let lemma_sub_same_public ts ins s1 s2 fuel =
+  let b, ts' = check_if_ins_consumes_fixed_time ins ts in
   let i, dsts, srcs = ins.ops in
   let r1 = taint_eval_ins ins s1 in
   let r2 = taint_eval_ins ins s2 in
@@ -142,12 +148,12 @@ let lemma_sub_same_public ts fuel ins s1 s2 =
 	  lemma_frame_store_mem64 ptr2 v2 s2.state.mem;
 	  assert (b2t b /\ r1.state.ok /\ r2.state.ok /\ publicValuesAreSame ts s1 s2 ==> publicValuesAreSame ts' r1 r2)
 
-val lemma_imul_same_public: (ts:taintState) -> (fuel:nat) -> (ins:tainted_ins{let i, _, _ = ins.ops in IMul64? i}) -> (s1:traceState) -> (s2:traceState) -> Lemma
-(let b, ts' = check_if_ins_consumes_fixed_time ins fuel ts in
+val lemma_imul_same_public: (ts:taintState) -> (ins:tainted_ins{let i, _, _ = ins.ops in IMul64? i}) -> (s1:traceState) -> (s2:traceState) -> (fuel:nat) -> Lemma
+(let b, ts' = check_if_ins_consumes_fixed_time ins ts in
   (b2t b ==> isExplicitLeakageFreeGivenStates (Ins ins) fuel ts ts' s1 s2))
 
-let lemma_imul_same_public ts fuel ins s1 s2 =
-  let b, ts' = check_if_ins_consumes_fixed_time ins fuel ts in
+let lemma_imul_same_public ts ins s1 s2 fuel =
+  let b, ts' = check_if_ins_consumes_fixed_time ins ts in
   let i, dsts, srcs = ins.ops in
   let r1 = taint_eval_ins ins s1 in
   let r2 = taint_eval_ins ins s2 in
@@ -173,12 +179,12 @@ let lemma_imul_same_public ts fuel ins s1 s2 =
 	  lemma_frame_store_mem64 ptr2 v2 s2.state.mem;
 	  assert (b2t b /\ r1.state.ok /\ r2.state.ok /\ publicValuesAreSame ts s1 s2 ==> publicValuesAreSame ts' r1 r2)
 
-val lemma_and_same_public: (ts:taintState) -> (fuel:nat) -> (ins:tainted_ins{let i, _, _ = ins.ops in And64? i}) -> (s1:traceState) -> (s2:traceState) -> Lemma
-(let b, ts' = check_if_ins_consumes_fixed_time ins fuel ts in
+val lemma_and_same_public: (ts:taintState) -> (ins:tainted_ins{let i, _, _ = ins.ops in And64? i}) -> (s1:traceState) -> (s2:traceState) -> (fuel:nat) -> Lemma
+(let b, ts' = check_if_ins_consumes_fixed_time ins ts in
   (b2t b ==> isExplicitLeakageFreeGivenStates (Ins ins) fuel ts ts' s1 s2))
 
-let lemma_and_same_public ts fuel ins s1 s2 =
-  let b, ts' = check_if_ins_consumes_fixed_time ins fuel ts in
+let lemma_and_same_public ts ins s1 s2 fuel =
+  let b, ts' = check_if_ins_consumes_fixed_time ins ts in
   let i, dsts, srcs = ins.ops in
   let r1 = taint_eval_ins ins s1 in
   let r2 = taint_eval_ins ins s2 in
@@ -204,12 +210,12 @@ let lemma_and_same_public ts fuel ins s1 s2 =
 	  lemma_frame_store_mem64 ptr2 v2 s2.state.mem;
 	  assert (b2t b /\ r1.state.ok /\ r2.state.ok /\ publicValuesAreSame ts s1 s2 ==> publicValuesAreSame ts' r1 r2)
 
-val lemma_addlea_same_public: (ts:taintState) -> (fuel:nat) -> (ins:tainted_ins{let i, _, _ = ins.ops in AddLea64? i}) -> (s1:traceState) -> (s2:traceState) -> Lemma
-(let b, ts' = check_if_ins_consumes_fixed_time ins fuel ts in
+val lemma_addlea_same_public: (ts:taintState) -> (ins:tainted_ins{let i, _, _ = ins.ops in AddLea64? i}) -> (s1:traceState) -> (s2:traceState) -> (fuel:nat) -> Lemma
+(let b, ts' = check_if_ins_consumes_fixed_time ins ts in
   (b2t b ==> isExplicitLeakageFreeGivenStates (Ins ins) fuel ts ts' s1 s2))
 
-let lemma_addlea_same_public ts fuel ins s1 s2 =
-  let b, ts' = check_if_ins_consumes_fixed_time ins fuel ts in
+let lemma_addlea_same_public ts ins s1 s2 fuel =
+  let b, ts' = check_if_ins_consumes_fixed_time ins ts in
   let i, dsts, srcs = ins.ops in
   let r1 = taint_eval_ins ins s1 in
   let r2 = taint_eval_ins ins s2 in
@@ -235,12 +241,12 @@ let lemma_addlea_same_public ts fuel ins s1 s2 =
 	  lemma_frame_store_mem64 ptr2 v2 s2.state.mem;
 	  assert (b2t b /\ r1.state.ok /\ r2.state.ok /\ publicValuesAreSame ts s1 s2 ==> publicValuesAreSame ts' r1 r2)
 
-val lemma_addcarry_same_public: (ts:taintState) -> (fuel:nat) -> (ins:tainted_ins{let i, _, _ = ins.ops in AddCarry64? i}) -> (s1:traceState) -> (s2:traceState) -> Lemma
-(let b, ts' = check_if_ins_consumes_fixed_time ins fuel ts in
+val lemma_addcarry_same_public: (ts:taintState) -> (ins:tainted_ins{let i, _, _ = ins.ops in AddCarry64? i}) -> (s1:traceState) -> (s2:traceState) -> (fuel:nat) -> Lemma
+(let b, ts' = check_if_ins_consumes_fixed_time ins ts in
   (b2t b ==> isExplicitLeakageFreeGivenStates (Ins ins) fuel ts ts' s1 s2))
 
-let lemma_addcarry_same_public ts fuel ins s1 s2 =
-  let b, ts' = check_if_ins_consumes_fixed_time ins fuel ts in
+let lemma_addcarry_same_public ts ins s1 s2 fuel =
+  let b, ts' = check_if_ins_consumes_fixed_time ins ts in
   let i, dsts, srcs = ins.ops in
   let r1 = taint_eval_ins ins s1 in
   let r2 = taint_eval_ins ins s2 in
@@ -268,23 +274,23 @@ let lemma_addcarry_same_public ts fuel ins s1 s2 =
 	  lemma_frame_store_mem64 ptr2 v2 s2.state.mem;
 	  assert (b2t b /\ r1.state.ok /\ r2.state.ok /\ publicValuesAreSame ts s1 s2 ==> publicValuesAreSame ts' r1 r2)
 
-val lemma_mul_same_public: (ts:taintState) -> (fuel:nat) -> (ins:tainted_ins{let i, _, _ = ins.ops in Mul64? i}) -> (s1:traceState) -> (s2:traceState) -> Lemma
-(let b, ts' = check_if_ins_consumes_fixed_time ins fuel ts in
+val lemma_mul_same_public: (ts:taintState) -> (ins:tainted_ins{let i, _, _ = ins.ops in Mul64? i}) -> (s1:traceState) -> (s2:traceState) -> (fuel:nat) -> Lemma
+(let b, ts' = check_if_ins_consumes_fixed_time ins ts in
   (b2t b ==> isExplicitLeakageFreeGivenStates (Ins ins) fuel ts ts' s1 s2))
 
-let lemma_mul_same_public ts fuel ins s1 s2 =
-  let b, ts' = check_if_ins_consumes_fixed_time ins fuel ts in
+let lemma_mul_same_public ts ins s1 s2 fuel =
+  let b, ts' = check_if_ins_consumes_fixed_time ins ts in
   let i, dsts, srcs = ins.ops in
   let r1 = taint_eval_ins ins s1 in
   let r2 = taint_eval_ins ins s2 in
   assert (b2t b /\ r1.state.ok /\ r2.state.ok /\ publicValuesAreSame ts s1 s2 ==> publicValuesAreSame ts' r1 r2)
 
-val lemma_shr_same_public: (ts:taintState) -> (fuel:nat) -> (ins:tainted_ins{let i, _, _ = ins.ops in Shr64? i}) -> (s1:traceState) -> (s2:traceState) -> Lemma
-(let b, ts' = check_if_ins_consumes_fixed_time ins fuel ts in
+val lemma_shr_same_public: (ts:taintState) -> (ins:tainted_ins{let i, _, _ = ins.ops in Shr64? i}) -> (s1:traceState) -> (s2:traceState) -> (fuel:nat) -> Lemma
+(let b, ts' = check_if_ins_consumes_fixed_time ins ts in
   (b2t b ==> isExplicitLeakageFreeGivenStates (Ins ins) fuel ts ts' s1 s2))
 
-let lemma_shr_same_public ts fuel ins s1 s2 =
-  let b, ts' = check_if_ins_consumes_fixed_time ins fuel ts in
+let lemma_shr_same_public ts ins s1 s2 fuel =
+  let b, ts' = check_if_ins_consumes_fixed_time ins ts in
   let i, dsts, srcs = ins.ops in
   let r1 = taint_eval_ins ins s1 in
   let r2 = taint_eval_ins ins s2 in
@@ -310,12 +316,12 @@ let lemma_shr_same_public ts fuel ins s1 s2 =
 	  lemma_frame_store_mem64 ptr2 v2 s2.state.mem;
 	  assert (b2t b /\ r1.state.ok /\ r2.state.ok /\ publicValuesAreSame ts s1 s2 ==> publicValuesAreSame ts' r1 r2)
 
-val lemma_shl_same_public: (ts:taintState) -> (fuel:nat) -> (ins:tainted_ins{let i, _, _ = ins.ops in Shl64? i}) -> (s1:traceState) -> (s2:traceState) -> Lemma
-(let b, ts' = check_if_ins_consumes_fixed_time ins fuel ts in
+val lemma_shl_same_public: (ts:taintState) -> (ins:tainted_ins{let i, _, _ = ins.ops in Shl64? i}) -> (s1:traceState) -> (s2:traceState) -> (fuel:nat) -> Lemma
+(let b, ts' = check_if_ins_consumes_fixed_time ins ts in
   (b2t b ==> isExplicitLeakageFreeGivenStates (Ins ins) fuel ts ts' s1 s2))
 
-let lemma_shl_same_public ts fuel ins s1 s2 =
-  let b, ts' = check_if_ins_consumes_fixed_time ins fuel ts in
+let lemma_shl_same_public ts ins s1 s2 fuel =
+  let b, ts' = check_if_ins_consumes_fixed_time ins ts in
   let i, dsts, srcs = ins.ops in
   let r1 = taint_eval_ins ins s1 in
   let r2 = taint_eval_ins ins s2 in
@@ -341,18 +347,18 @@ let lemma_shl_same_public ts fuel ins s1 s2 =
 	  lemma_frame_store_mem64 ptr2 v2 s2.state.mem;
 	  assert (b2t b /\ r1.state.ok /\ r2.state.ok /\ publicValuesAreSame ts s1 s2 ==> publicValuesAreSame ts' r1 r2)
 
-val lemma_xor_same_public: (ts:taintState) -> (fuel:nat) -> (ins:tainted_ins{let i, _, _ = ins.ops in Xor64? i}) -> (s1:traceState) -> (s2:traceState) -> Lemma
-(let b, ts' = check_if_ins_consumes_fixed_time ins fuel ts in
+val lemma_xor_same_public: (ts:taintState) -> (ins:tainted_ins{let i, _, _ = ins.ops in Xor64? i}) -> (s1:traceState) -> (s2:traceState) -> (fuel:nat) -> Lemma
+(let b, ts' = check_if_ins_consumes_fixed_time ins ts in
   (b2t b ==> isExplicitLeakageFreeGivenStates (Ins ins) fuel ts ts' s1 s2))
 
 val lemma_aux_xor: (x:nat64) -> Lemma (Types_s.ixor x x = 0)
 
-let lemma_aux_xor x =
+let lemma_aux_xor x = 
   TypesNative_s.reveal_ixor 64 x x;
   FStar.UInt.logxor_self #64 x
 
-let lemma_xor_same_public ts fuel ins s1 s2 =
-  let b, ts' = check_if_ins_consumes_fixed_time ins fuel ts in
+let lemma_xor_same_public ts ins s1 s2 fuel =
+  let b, ts' = check_if_ins_consumes_fixed_time ins ts in
   let i, dsts, srcs = ins.ops in
   let r1 = taint_eval_ins ins s1 in
   let r2 = taint_eval_ins ins s2 in
@@ -380,31 +386,31 @@ let lemma_xor_same_public ts fuel ins s1 s2 =
 	  assert (b2t b /\ r1.state.ok /\ r2.state.ok /\ publicValuesAreSame ts s1 s2 ==> publicValuesAreSame ts' r1 r2)
 
 #reset-options "--initial_ifuel 2 --max_ifuel 2 --initial_fuel 4 --max_fuel 4 --using_facts_from '* -FStar.Reflection -FStar.Tactics' --z3rlimit 20"
-val lemma_ins_same_public: (ts:taintState) -> (fuel:nat) -> (ins:tainted_ins{not (is_xmm_ins ins)}) -> (s1:traceState) -> (s2:traceState) -> Lemma
-(let b, ts' = check_if_ins_consumes_fixed_time ins fuel ts in
+val lemma_ins_same_public: (ts:taintState) -> (ins:tainted_ins{not (is_xmm_ins ins)}) -> (s1:traceState) -> (s2:traceState) -> (fuel:nat) -> Lemma
+(let b, ts' = check_if_ins_consumes_fixed_time ins ts in
   (b2t b ==> isExplicitLeakageFreeGivenStates (Ins ins) fuel ts ts' s1 s2))
 
-let lemma_ins_same_public ts fuel ins s1 s2 = let i, _, _ = ins.ops in
+let lemma_ins_same_public ts ins s1 s2 fuel = let i, _, _ = ins.ops in
   match i with
-  | Mov64 _ _ -> lemma_mov_same_public ts fuel ins s1 s2
-  | Add64 _ _ -> lemma_add_same_public ts fuel ins s1 s2
-  | AddLea64 _ _ _ -> lemma_addlea_same_public ts fuel ins s1 s2
-  | Sub64 _ _ -> lemma_sub_same_public ts fuel ins s1 s2
-  | IMul64 _ _ -> lemma_imul_same_public ts fuel ins s1 s2
-  | And64 _ _ -> lemma_and_same_public ts fuel ins s1 s2
-  | Mul64 _ -> lemma_mul_same_public ts fuel ins s1 s2
-  | Xor64 _ _ -> lemma_xor_same_public ts fuel ins s1 s2
-  | AddCarry64 _ _ -> lemma_addcarry_same_public ts fuel ins s1 s2
-  | Shl64 _ _ -> lemma_shl_same_public ts fuel ins s1 s2
-  | Shr64 _ _ -> lemma_shr_same_public ts fuel ins s1 s2
+  | Mov64 _ _ -> lemma_mov_same_public ts ins s1 s2 fuel
+  | Add64 _ _ -> lemma_add_same_public ts ins s1 s2 fuel
+  | AddLea64 _ _ _ -> lemma_addlea_same_public ts ins s1 s2 fuel
+  | Sub64 _ _ -> lemma_sub_same_public ts ins s1 s2 fuel
+  | IMul64 _ _ -> lemma_imul_same_public ts ins s1 s2 fuel
+  | And64 _ _ -> lemma_and_same_public ts ins s1 s2 fuel
+  | Mul64 _ -> lemma_mul_same_public ts ins s1 s2 fuel
+  | Xor64 _ _ -> lemma_xor_same_public ts ins s1 s2 fuel
+  | AddCarry64 _ _ -> lemma_addcarry_same_public ts ins s1 s2 fuel
+  | Shl64 _ _ -> lemma_shl_same_public ts ins s1 s2 fuel
+  | Shr64 _ _ -> lemma_shr_same_public ts ins s1 s2 fuel
 
-val lemma_ins_leakage_free: (ts:taintState) -> (fuel:nat) -> (ins:tainted_ins{not (is_xmm_ins ins)}) -> Lemma
- (let b, ts' = check_if_ins_consumes_fixed_time ins fuel ts in
-  (b2t b ==> isConstantTime (Ins ins) fuel ts /\ isLeakageFree (Ins ins) fuel ts ts'))
+val lemma_ins_leakage_free: (ts:taintState) -> (ins:tainted_ins{not (is_xmm_ins ins)}) -> Lemma
+ (let b, ts' = check_if_ins_consumes_fixed_time ins ts in
+  (b2t b ==> isConstantTime (Ins ins) ts /\ isLeakageFree (Ins ins) ts ts'))
 
-let lemma_ins_leakage_free ts fuel ins =
-  let b, ts' = check_if_ins_consumes_fixed_time ins fuel ts in
-  let p s1 s2 = b2t b ==> isExplicitLeakageFreeGivenStates (Ins ins) fuel ts ts' s1 s2 in
-  let my_lemma s1 s2 : Lemma(p s1 s2) = lemma_ins_same_public ts fuel ins s1 s2 in
+let lemma_ins_leakage_free ts ins =
+  let b, ts' = check_if_ins_consumes_fixed_time ins ts in
+  let p s1 s2 fuel = b2t b ==> isExplicitLeakageFreeGivenStates (Ins ins) fuel ts ts' s1 s2 in
+  let my_lemma s1 s2 fuel : Lemma(p s1 s2 fuel) = lemma_ins_same_public ts ins s1 s2 fuel in
   let open FStar.Classical in
-  forall_intro_2 my_lemma
+  forall_intro_3 my_lemma
